test/Compiler.v
@@ -1,6 +1,13 @@
 Require Import CoqCompile.Compile.
 Require Import LLVM.
 Require Import Lambda.
+Require Import String.
+Require Import ExtLib.Programming.Show.
 
-Definition result : Compile.m LLVM.module :=
-  Compile.topCompile 8 Compile.Opt.O0 true (LambdaNotation.gen LambdaNotation.e8) Compile.LLVM_stop false.
+Definition result (* : Compile.m LLVM.module*) :=
+  match 
+    Compile.runM (Compile.topCompile 8 Compile.Opt.O0 true (LambdaNotation.gen LambdaNotation.e8) Compile.LLVM_stop false)
+    with
+    | (inr m, _) => to_string m
+    | _ => "error"%string
+  end.
